raft first draft

raft/simulator/lib/Simulator.ml
@@ -1,45 +1,59 @@
-open Colors
-open Prelude
-open RsaKeyFun
 open Core
 
-(* the generic type *)
+(* This module defines the abstract type classes and basic functions
+   to easily implement a simulator for some protocol.
+   Maybe it would be usefull to provide an .mli file
+
+   The classes uses generic types which can lead to confusions
+   or maybe inappropriate in complex cases.
+
+   The rough method is to implement the virtual methods of the simulator class
+   which should be sufficient for ocaml to guess the types and run the simulation.
+*)
+
+(* handy print functions with colored output *)
+(* print error messages *)
+let print_err msg =
+  print_endline (Colors.kBRED ^ "Error:\t[" ^ msg ^ "]" ^ Colors.kNRM)
+
+(* print info messages with c - color; t - message type; msg - message *)
+let print_info c t msg =
+  print_endline (c ^ "Info:\t{" ^ t ^ ": " ^ msg ^ "}" ^ Colors.kNRM)
+
+(* print results t - timestamp; d - elapsed time; avg - average *)
+let print_res t d avg  =
+  print_endline (Colors.kMAG ^ "Result:\t[Timestamp: " ^ string_of_int t
+                 ^ "; elapsed time: " ^ (Batteries.String.of_list (Prelude.Time.time2string d))
+                 ^ "; average: " ^ Batteries.String.of_list (Prelude.Time.time2string avg)
+                 ^ "]" ^ Colors.kNRM)
+
+(* The basic record which connects an id with some replica.
+   The semantic is mostly that the id the the node name and
+   the replica is some sort of current state. *)
 type ('a, 'b) idrep = { id : 'a ; replica : 'b }
 
-(* create a list of replicas *)
+(* This is the basic object for working with replicas. *)
 class ['a, 'b] replicas = object(self)
   val mutable r : ('a, 'b) idrep list ref = ref []
 
-  (* assign replicas *)
+  (* assign a list of replicas *)
   method set_replicas (l : ('a, 'b) idrep list) =
     r := l
 
+  (* get all replicas *)
   method get_replicas : ('a, 'b) idrep list =
     !r
 
+  (* return some replica iff the id is found *)
   method find_replica id : ('a, 'b) idrep option =
     List.find ~f:(fun x -> id = x.id) !r
 
+  (* replace the current replica with a new one *)
   method replace_replica id rep : unit =
     r := List.map ~f:(fun x -> if id = x.id then { id = id; replica = rep } else x) !r
 end
 
-(* print error messages *)
-let print_err msg =
-  print_endline (kBRED ^ "Error:\t[" ^ msg ^ "]" ^ kNRM)
-
-(* print info messages with c - color; t - message type; msg - message *)
-let print_info c t msg =
-  print_endline (c ^ "Info:\t{" ^ t ^ ": " ^ msg ^ "}" ^ kNRM)
-
-(* print results t - timestamp; d - elapsed time; avg - average *)
-let print_res t d avg  =
-  print_endline (kMAG ^ "Result:\t[Timestamp: " ^ string_of_int t
-                 ^ "; elapsed time: " ^ (Batteries.String.of_list (Prelude.Time.time2string d))
-                 ^ "; average: " ^ Batteries.String.of_list (Prelude.Time.time2string avg)
-                 ^ "]" ^ kNRM)
-
-
+(* A basic run configuration *)
 type ('a) run_conf = {
   version : string;
   protocol : string;
@@ -48,8 +62,12 @@ type ('a) run_conf = {
   primary : 'a;
 }
 
-class virtual ['a, 'b] runner c = object(self)
+(* the abstract simulator provides convient functions to implement a new protocol.
+   Inherit and implement the virtual methods. See PbSimul.ml and PbftSimul.ml as reference
+   'a -> Nodename ; 'b -> protocol message ; 'c -> directed message type ; 'd -> state machine *)
+class virtual ['a, 'b, 'c, 'd] simulator c = object(self)
   val mutable conf : ('a) run_conf = c
+  val mutable replicas : ('a, 'd) replicas = new replicas
 
   (** create all the replicas **)
   method virtual create_replicas : unit
@@ -57,21 +75,24 @@ class virtual ['a, 'b] runner c = object(self)
   (** specify how some client request is made **)
   method virtual mk_request : int -> int -> 'b
 
+  (** specify how the replica handles input messages **)
+  method virtual run_replicas : 'c -> 'c
+
   (** specify the client **)
   method virtual run_client : int -> int -> Prelude.Time.t -> int -> unit
 
   (* maybe this could be more generalized *)
   (** An implementation should catch the spec args <max> <printing_period> initialize the crypto;
       set the replicas and at last call run_client **)
-  method callback : int -> int -> unit -> unit =
-    (fun max printing_period () ->
-       print_info (kBLU) "Main" "Initialize random generator";
+  method callback : int -> int -> bool -> unit -> unit =
+    (fun max printing_period debug () ->
+       print_info (Colors.kBLU) "Main" "Initialize random generator";
        let () = Nocrypto_entropy_unix.initialize () in
 
-       print_info (kBLU) "Main" "Start replicas";
+       print_info (Colors.kBLU) "Main" "Start replicas";
        self#create_replicas;
 
-       print_info (kBLU) "Main" "Fire up client";
+       print_info (Colors.kBLU) "Main" "Fire up client";
        let initial_timestamp = 1 in
        let initial_avg       = Prelude.Time.mk_time 0. in
        self#run_client initial_timestamp max initial_avg printing_period)
@@ -89,12 +110,14 @@ class virtual ['a, 'b] runner c = object(self)
 
         +> flag "-printing-period" (optional_with_default 10 int)
           ~doc:" Number of messages till a summary is printed (default 10)"
+        +> flag "-debug" (optional_with_default true bool)
+          ~doc: "Verbose output (default true)"
       )
       self#callback
 
   (** run a simulator with some specified configuration **)
   method run =
-    print_info (kWHT) "Main" ("Running simulator for " ^ conf.protocol
+    print_info (Colors.kWHT) "Main" ("Running simulator for " ^ conf.protocol
                               ^ " Version: " ^ conf.version);
     Command.run ~version:conf.version ~build_info:conf.protocol self#spec
 end
