raft/protocols/Raft/Raft.v
@@ -3,8 +3,7 @@
  *)
 
 (* import velisarios *)
-Require Export Velisarios.Quorum.
-Require Export Velisarios.Process.
+Require Export Protocols.Raft.RaftHeader.
 Require Export String.
 Require Export Peano.
 Require Export List.
@@ -15,174 +14,91 @@ Section Raft.
   Local Open Scope eo.
   Local Open Scope proc.
 
-  (* define a context configuration for all nodes *)
-  Class Raftcontext :=
-    MkRaftContext
-      {
-        (* define the amount of clients and the bijective homomorphism  *)
-        clients : nat;
-        C : Set;
-        client_deq : Deq C;
-        clients2nat : C -> nat_n clients;
-        clients_bji : bijective clients2nat;
+  Context { raft_context : RaftContext }.
 
-        (* define the amount of replicas by num faults and the bijective homomorphism *)
-        F : nat;
-        reps := (3 * F) + 1;
-        Rep : Set;
-        rep_deq : Deq Rep;
-        reps2nat : Rep -> nat_n reps;
-        reps_bij : bijective reps2nat;
+  (* ++++++++++++++ Primary state ++++++++++++++ *)
+  Record RaftPrimaryState :=
+    Build_Primary_State
+      {
+        (* store the current node term number *)
+        term_number_prim : Term;
       }.
 
-  Context { raft_context : Raftcontext }.
+  (* define the initial state for the primary *)
+  Definition initial_primary_state : RaftPrimaryState :=
+    Build_Primary_State
+      initial_term.
 
-  (* define the node types *)
-  Inductive Raftnode :=
-  (* handles client io, issues log replication max 1 *)
-  | Replica (n : Rep)
-  (* issue state change requests *)
-  | Client (n : C).
+  (* ++++++++++++++ State ++++++++++++++
+   * This record describe the general state of all nodes
+   * in the system. *)
+  Record RaftState :=
+    Build_State
+      {
+        (* store the current node term number *)
+        term_number : Term;
+        (* the local state machine *)
+        sm_state : RaftSM_state;
+        (* the timeout in secs after which a new election is triggered *)
+        timeout : nat;
+        (* indicate if this node is the leader *)
+        leader : bool;
+      }.
 
-  (* prove decidable equality for the nodes *)
-  Lemma Deq_Raftnode : Deq Raftnode.
-  Proof.
-    introv; destruct x as [r1|c1], y as [r2|c2].
-    + destruct (rep_deq r1 r2); [left|right]; subst; auto.
-      intro xx; inversion xx; subst; tcsp.
-    + right; intro xx; inversion xx; subst; tcsp.
-    + right; intro xx; inversion xx; subst; tcsp.
-    + destruct (client_deq c1 c2); [left|right]; subst; auto.
-      intro xx; inversion xx; subst; tcsp.
-  Qed.
+  (* define the first state of some node *)
+  Definition initial_state (r : Rep) : RaftState :=
+    Build_State
+      initial_term
+      RaftSM_initial_state
+      5
+      false.
 
-  Global Instance Raft_I_Node : Node := MkNode Raftnode Deq_Raftnode.
+  (* increment the term number *)
+  Definition increment_term_num (s : RaftState) : RaftState :=
+    Build_State
+      (next_term (term_number s))
+      (sm_state s)
+      (timeout s)
+      (leader s).
 
-  (* define the quorum context *)
-  Lemma Replica_inj : injective Replica.
-  Proof.
-    introv h; ginv; auto.
-  Qed.
+  (* ++++++++++++++ Update functions ++++++++++++++ *)
+  (* handle input - currently by doing nothing *)
+  Definition Rafthandle_input (slf : Rep) : Update RaftState nat DirectedMsgs :=
+    fun state i => (Some state, []).
 
-  Global Instance Raft_I_Quorum : Quorum_context :=
-    MkQuorumContext
-      Rep
-      reps
-      rep_deq
-      reps2nat
-      reps_bij
-      Replica
-      Replica_inj.
+  (* handle heartbeat by reseting the timer *)
+  Definition Rafthandle_heartbeat (slf : Rep) : Update RaftState unit DirectedMsgs :=
+    fun state _ => (Some state, []).
 
-  Definition rep2node := Rep -> node_type.
-
-
-
-
-
-  Inductive Raftmsg :=
-  (* the leader signals it's alive *)
-  | Heartbeat
-  (* reply the new term number to the client *)
-  | Reply (new_term_num : nat) (c : C)
-  (* the command issued by the client - here new term number *)
-  | Command (term_num : nat).
-
-  Global Instance Raft_I_Msg : Msg := MkMsg Raftmsg.
-
-  Definition Raft_msg_status (m : msg) : msg_status :=
-    match m with
-    (* flag the heartbeat msg as system internal message *)
-    | Heartbeat => MSG_STATUS_INTERNAL
-    (* the outgoing reply to the client is set to internal? *)
-    | Reply _ _ => MSG_STATUS_INTERNAL
-    (* flag the command msg as from outside the system *)
-    | Command _ => MSG_STATUS_EXTERNAL
-    end.
-
-  Global Instance Raft_I_MsgStatus : MsgStatus := MkMsgStatus Raft_msg_status.
-
-  (* receive a message from the client and extract the number *)
-  Definition receive_command (m : Raftmsg) : option nat :=
-    match m with
-    | Command n => Some n
-    | _ => None
-    end.
-
-  Definition send_command (n : nat) (names : list name) : DirectedMsg :=
-    MkDMsg (Command n) names 0.
-
-  Inductive Raftleader_state :=
-    (* the current term of the global network *)
-  | Term (term_num : nat).
-
-  (* define the update function of the leader *)
-  Definition leader_update : MSUpdate Raftleader_state :=
-    fun state input =>
-      match state, input with
-      (* update the term_num and reply to the client *)
-      | Term n, Command m => (Term m, [])
-      (* ignore other messages *)
-      | _, _ => (state, [])
+  (* Define the update function which is executed within the state machines *)
+  Definition Raftreplica_update (slf : Rep) : MUpdate RaftState :=
+    fun state m =>
+      match m with
+      | Input n => Rafthandle_input slf state n
+      | Heartbeat => Rafthandle_heartbeat slf state tt
       end.
 
-  (* initialize the state machines ? *)
-  Arguments MkSM      [S] [I] [O] _ _ _.
-  Arguments sm_halted [S] [I] [O] _.
-  Arguments sm_state  [S] [I] [O] _.
-  Arguments sm_update [S] [I] [O] _ _ _.
 
-  (* initialize the leader state machine *)
-  Definition RaftleaderSM : MStateMachine Raftleader_state :=
-    mkSSM leader_update (Term 0).
+  (* ++++++++++++++ System ++++++++++++++
+   * Define the actual state machines and hook them into velisarios. *)
+  Definition RaftreplicaSM (slf : Rep) : MStateMachine _ (* let the compiler guess ? *) :=
+    mkSM
+      (Raftreplica_update slf)
+      (initial_state slf).
 
-  (* link the node name to the state definition *)
-  Definition Raftstate (n : name) :=
+  (* match node names with state machines *)
+  Definition Raftnstate (n : name) :=
     match n with
-    | Raftleader => Raftleader_state
+    | Raftreplica _ => RaftState
+    | _ => unit
     end.
 
-  (* link the node name with the state ?? *)
-  Definition Raftusys : MUSystem Raftstate :=
+  Definition Raftsys : MUSystem Raftnstate :=
     fun name =>
-      match name return StateMachine (Raftstate name) msg DirectedMsgs with
-      | Raftleader => RaftleaderSM
+      match name return StateMachine (Raftnstate name) msg DirectedMsgs with
+      | Raftreplica n => RaftreplicaSM n
+      | _ => MhaltedSM tt
       end.
-
-  Definition Raftsys : System :=
-    fun name =>
-      match name with
-      | Raftleader => build_sprocess leader_update (Term 0)
-      end.
-
-  (* authencation interfaces *)
-  Instance Raft_I_Key : Key := MkKey unit unit.
-
-  Instance Raft_I_Data : Data := MkData Raftmsg.
-
-  Instance Raft_I_AuthTok : AuthTok := MkAuthTok unit Deq_unit.
-
-  Instance Raft_I_AuthFun : AuthFun :=
-    MkAuthFun
-      (fun _ _ => [tt])
-      (fun _ _ _ _ => true).
-
-  (* authenticate data, match messages with nodes which issued them
-   * ignore n since nobody sents a message to itself *)
-  (* Definition Raftdata_auth : name -> Raftmsg -> option name := *)
-  (*   fun n m => *)
-  (*     match m with *)
-  (*     | Heartbeat => Some Replica *)
-  (*     | Reply _ _ => Some Replica *)
-  (*     | Command _ => Some Client *)
-  (*     end. *)
-
-  (* (* link authentication function to the abstract authenticated data type *) *)
-  (* Instance Raft_I_DataAuth : DataAuth := MkDataAuth Raftdata_auth. *)
-
-  (* (* create nested authdata; tt indicates that the data is authenticated *) *)
-  (* Instance Raft_I_ContainedAuthData : ContainedAuthData := *)
-  (*   MkContainedAuthData (fun m => [MkAuthData m [tt]]). *)
 
   (* tactic hints ? *)
   (* QUESTION: Can we avoid repeating this? *)
