raft/protocols/Raft/RaftHeader.v
@@ -1,0 +1,143 @@
+(*
+ * This is the header file defining the basics of the raft
+ * protocol with velisarios.
+ *)
+
+(* find what the quorum file defines, maybe not needed? *)
+Require Export Velisarios.Quorum.
+Require Export Velisarios.Process.
+
+Section RaftHeader.
+
+  (* needed? *)
+  Local Open Scope eo.
+  Local Open Scope proc.
+
+  (* define the basic context which is included into the raft replicas *)
+  Class RaftContext :=
+    MkRaftContext
+      {
+        (* number of faults *)
+        F : nat;
+        (* number of replicas needed *)
+        num_replicas := (3 * F) + 1;
+        (* the replicas are only some type *)
+        Rep : Set;
+        (* replicas have decidable equality *)
+        rep_deq : Deq Rep;
+        (* replicas can be associated with some natural number *)
+        reps2nat : Rep -> nat_n num_replicas;
+        (* the projection is bijective; bijective is defined in Quorum *)
+        reps_bij : bijective reps2nat;
+        (* the number of clients allowed *)
+        num_clients : nat;
+        (* clients are just some ordenary type *)
+        Client : Set;
+        (* clients have decidable equality *)
+        client_deq : Deq Client;
+        (* clients can be associated with some number *)
+        clients2nat : Client -> nat_n num_clients;
+        (* the projections ist bijective *)
+        clients_bij : bijective clients2nat;
+        (* describe the local state machines *)
+        RaftSM_state : Set;
+        (* the initial state of the state machine *)
+        RaftSM_initial_state : RaftSM_state;
+      }.
+
+  Context { raft_context : RaftContext }.
+
+  (* define the node types with the arbitrary types defined in the context *)
+  Inductive Raftnode :=
+  | Raftreplica (n : Rep)
+  | Raftclient (n : Client).
+
+  (* extract the replica of some node *)
+  Definition node2rep (n : Raftnode) : option Rep :=
+    match n with
+    | Raftreplica n => Some n
+    | _ => None
+    end.
+
+  (* extract the client of some node *)
+  Definition client2rep (n : Raftnode) : option Client :=
+    match n with
+    | Raftclient n => Some n
+    | _ => None
+    end.
+
+  (* prove that some raft node has decidable equality *)
+  Lemma RaftnodeDeq : Deq Raftnode.
+  Proof.
+    introv.
+    destruct x as [r1|c1], y as [r2|c2].
+    + destruct (rep_deq r1 r2); [left|right]; subst; auto.
+      intro xx. inversion xx. subst. tcsp.
+    + right; intro xx. inversion xx; subst.
+    + right; intro xx. inversion xx; subst.
+    + destruct (client_deq c1 c2); [left|right]; subst; auto.
+      intro xx. inversion xx. subst. tcsp.
+  Defined.
+
+  Global Instance Raft_I_Node : Node := MkNode Raftnode RaftnodeDeq.
+
+  (* ++++++++++++++ Terms ++++++++++++++
+   * Terms are the progress steps of the protocol.
+   * A term consists of a full round-trip through the system
+   * and ends with an agreement of some new state of the system.
+   * Also if some difference or failure happens within the system
+   * the last terms are rolled back to get the last valid state.
+   *)
+  Inductive Term := term (n : nat).
+
+  Definition term2nat (t : Term) : nat :=
+    match t with
+    | term n => n
+    end.
+  (* define that the term type and nat type are interchangable  *)
+  Coercion term2nat : Term >-> nat.
+
+  (* define the term succsessor *)
+  Definition next_term (t : Term) : Term := term (S t).
+  (* define the term predecessor *)
+  Definition pred_term (t : Term) : Term := term (pred t).
+
+  (* prove that terms are decidable *)
+  Lemma TermDeq : Deq Term.
+  Proof.
+    introv. destruct x, y; prove_dec.
+    destruct (deq_nat n n0); prove_dec.
+  Defined.
+
+  (* define the initial term *)
+  Definition initial_term := term 0.
+
+  (* define lesser or equal for two terms *)
+  Definition TermLe (t1 t2 : Term) : bool :=
+    term2nat t1 <=? term2nat t2.
+
+  (* define lesser for two terms *)
+  Definition TermLt (t1 t2 : Term) : bool :=
+    term2nat t1 <? term2nat t2.
+
+  (* find the greater term *)
+  Definition max_term (t1 t2 : Term) : Term :=
+    if TermLe t1 t2 then t2 else t1.
+
+  (* ++++++++++++++ Messsages ++++++++++++++ *)
+  Inductive Raftmsg :=
+  | Input (n : nat)
+  | Heartbeat.
+
+  Global Instance Raft_I_Msg : Msg := MkMsg Raftmsg.
+
+  Definition Raftmsg2status (m : Raftmsg) : msg_status :=
+    match m with
+    | Input _ => MSG_STATUS_EXTERNAL
+    | Heartbeat => MSG_STATUS_INTERNAL
+    end.
+
+  Global Instance Raft_I_get_msg_status : MsgStatus := MkMsgStatus Raftmsg2status.
+
+
+End RaftHeader.
